src/tls/Signature.fst
@@ -1,0 +1,328 @@
+module Signature
+
+open FStar.Monotonic.RRef
+open FStar.HyperHeap
+open Platform.Bytes
+
+open MonotoneSeq
+open TLSConstants
+open CoreCrypto
+
+
+(* ------------------------------------------------------------------------ *)
+type text = bytes
+
+type alg =
+  | Use: info:(text -> Type0)
+       -> core: sigAlg
+       -> digest: list hashAlg
+       -> keyEncipher: bool // can encrypt e.g. PMS in TLS_RSA_WITH_...
+       -> keyExchange: bool // can be used to establish a Diffie-Hellman secret e.g. in TLS_DH_... SZ: Do we care about static (EC)DH?
+       -> alg
+
+type signed (a:alg) = t:text{a.info t}
+
+// Could be finer, but we lack lengths in CoreCrypto signature functions
+type sigv (a:alg) = bytes
+
+// controls idealization of Sig
+let ideal = IdealFlags.ideal_Sig
+
+// Encodes agile INT-CMA assumption
+assume type int_cma: a:alg -> h:hashAlg{List.Tot.mem h a.digest} -> Tot bool
+
+type public_repr = 
+  | PK_RSA   of rsa_key
+  | PK_DSA   of dsa_key
+  | PK_ECDSA of ec_key
+
+type secret_repr =
+  | SK_RSA   of rsa_key
+  | SK_DSA   of dsa_key
+  | SK_ECDSA of ec_key
+
+let sigAlg_of_secret_repr sk =
+  match sk with
+  | SK_RSA k -> RSASIG // Ignore RSA-PSS
+  | SK_DSA k -> DSA
+  | SK_ECDSA k -> ECDSA
+
+let sigAlg_of_public_repr pk =
+  match pk with
+  | PK_RSA k   -> RSASIG // Ignore RSA-PSS
+  | PK_DSA k   -> DSA
+  | PK_ECDSA k -> ECDSA
+
+private val sig_digest: hashAlg -> bytes -> Tot (option hash_alg * bytes)
+let sig_digest h t =
+  match h with
+  | NULL    -> None, t
+  | MD5SHA1 -> None, HASH.hash h t
+  | Hash h  -> Some h, t
+
+
+(* ------------------------------------------------------------------------ *)
+type state (a:alg) =
+  | Signed: log:Seq.seq (signed a) -> state a
+  | Corrupt
+
+(* 
+  Allowed state transitions:
+  Corrupt  -> Corrupt
+  Signed l -> Corrupt
+  Signed l -> Signed l++l'
+*)
+abstract let evolves (#a:alg) (s1:state a) (s2:state a) =
+  is_Corrupt s2 \/ 
+  (is_Signed s1 /\ is_Signed s2 /\ grows (Signed.log s1) (Signed.log s2))
+
+let lemma_evolves_monotone (#a:alg): Lemma (monotonic (state a) (evolves #a)) = 
+  forall_intro (seq_extension_reflexive #(signed a));
+  forall_intro_3 (grows_transitive #(signed a))
+
+private val st_update: #a:alg 
+  -> s1:state a 
+  -> signed a 
+  -> Tot (s2:state a{evolves s1 s2})
+let st_update #a st t =
+  match st with
+  | Signed ts -> Signed (snoc ts t)
+  | Corrupt   -> Corrupt
+
+
+(* ------------------------------------------------------------------------ *)
+assume val keyRegion: rid
+
+type log_t (a:alg) = m_rref keyRegion (state a) evolves
+
+type pubkey (a:alg) =
+  | PK: log:log_t a -> repr:public_repr{sigAlg_of_public_repr repr = a.core} -> pubkey a
+
+type pkey = (a:alg & pubkey a)
+
+val pkey_repr: pkey -> Tot public_repr
+let pkey_repr (| a,  p |) = PK.repr p
+
+type skey (a:alg) = 
+  k:(pubkey a * secret_repr){let _,sk = k in sigAlg_of_secret_repr sk = a.core}
+
+val alloc_pubkey: #a:alg
+  -> s:state a 
+  -> r:public_repr{sigAlg_of_public_repr r = a.core}
+  -> ST (pubkey a)
+    (requires (fun h0 -> True))
+    (ensures  (fun h0 p h1 -> ralloc_post keyRegion s h0 (as_rref (PK.log p)) h1
+                           /\ PK.repr p = r
+                           /\ m_fresh (PK.log p) h0 h1))
+let alloc_pubkey #a s r =
+  lemma_evolves_monotone #a;
+  let log = m_alloc keyRegion s in 
+  PK log r
+
+
+(* ------------------------------------------------------------------------ *)
+(* We rely on key-generation producing pairwise-distinct public keys
+  with overwhelming probability. This follows from any crypto
+  security assumptions, and most reasonable generation algorithms;
+  we might not record keys generated with hopeless algorithms.
+
+  We maintain this property as a stateful invariaint in rkeys *)
+
+type kset = s:list pkey{ forall x y. (List.Tot.mem x s /\ List.Tot.mem y s /\ pkey_repr x = pkey_repr y) ==> x = y }
+
+val find_key: r:public_repr -> ks: kset 
+  -> Tot (o:option (k:pkey {pkey_repr k = r && List.Tot.mem k ks})
+        { is_None o ==> (forall k. List.Tot.mem k ks ==> pkey_repr k <> r) })
+let rec find_key r ks = match ks with
+  | []   -> None
+  | k::ks -> if pkey_repr k = r then Some k else find_key r ks
+
+val add_key: ks:kset 
+  -> k:pkey { forall k'. List.Tot.mem k' ks ==> pkey_repr k <> pkey_repr k' } 
+  -> Tot kset
+let add_key ks k = k::ks
+
+unfoldable logic type mon_pkey (xs:kset) (xs':kset) =
+  forall x. List.Tot.mem x xs ==> List.Tot.mem x xs'
+
+// FIXME: top-level effect
+val rkeys: m_rref keyRegion kset (mon_pkey)
+let rkeys = m_alloc keyRegion []
+
+type generated (k:pkey) (h:HyperHeap.t) : Type0 = List.Tot.mem k (m_sel h rkeys)
+
+
+(* ------------------------------------------------------------------------ *)
+val sign: #a:alg
+  -> h:hashAlg{List.Tot.mem h (a.digest)} 
+  -> s:skey a 
+  -> t:signed a 
+  -> ST (sigv a)
+    (requires (fun h -> True))
+    (ensures  (fun h0 _ h1 ->
+      if ideal then
+        let (pk,sk) = s in 
+        let log = PK.log pk in
+        modifies (Set.singleton keyRegion) h0 h1 /\
+        m_sel h1 log == st_update (m_sel h0 log) t 
+      else modifies Set.empty h0 h1))
+
+let sign #a h s t =
+  let (pk,sk) = s in
+  begin
+  if ideal then
+    let log = PK.log pk in
+    let s0 = m_read log in
+    m_write log (st_update s0 t)
+  end;
+  let ho,t' = sig_digest h t in
+  let signature =
+    match sk with
+    | SK_RSA k   -> rsa_sign ho k t'
+    | SK_DSA k   -> dsa_sign ho k t'
+    | SK_ECDSA k -> ecdsa_sign ho k t'
+  in
+  signature
+
+
+(* ------------------------------------------------------------------------ *)
+val verify: #a:alg 
+  -> h:hashAlg{List.Tot.mem h (a.digest)} 
+  -> pk:pubkey a 
+  -> t:text
+  -> sigv a
+  -> ST bool
+    (requires (fun h -> True))
+    (ensures  (fun h0 b h1 -> 
+	           modifies Set.empty h0 h1
+		 /\ (b /\ ideal
+		    /\ List.Tot.existsb (fun (k:pkey) -> let (|_,pk'|) = k in pk = pk') (m_sel h0 rkeys)
+		    /\ int_cma a h
+		    /\ is_Signed (m_sel h0 (PK.log pk))) ==>
+		    a.info t))
+
+let verify #a h pk t s =
+  let verified =
+    let ho,t' = sig_digest h t in
+    match PK.repr pk with
+    | PK_RSA k   -> rsa_verify ho k t' s
+    | PK_DSA k   -> dsa_verify ho k t' s
+    | PK_ECDSA k -> ecdsa_verify ho k t' s
+  in
+  if ideal then
+    let signed =
+      let log = m_read (PK.log pk) in
+      match log with
+      | Signed ts -> is_Some (SeqProperties.seq_find (fun (t':signed a) -> t = t') (Signed.log log))
+      | Corrupt   -> true
+    in
+    let honest =
+      let kset = m_read rkeys in
+      List.Tot.existsb (fun (k:pkey) -> let (|_,pk'|) = k in pk = pk') kset
+    in
+    verified && (signed || not (honest && int_cma a h))
+  else
+    verified
+
+
+(* ------------------------------------------------------------------------ *)
+val genrepr: a:alg 
+  -> All (public_repr * secret_repr)
+    (requires (fun h -> True))
+    (ensures  (fun h0 k h1 -> 
+      	is_V k ==>
+	(let (pk,sk) = V.v k in
+        modifies Set.empty h0 h1
+	/\ sigAlg_of_public_repr pk = sigAlg_of_secret_repr sk
+	/\ sigAlg_of_public_repr pk = a.core)))
+let genrepr a =
+  match a.core with
+  | RSASIG -> let k = rsa_gen_key 2048 in (PK_RSA k, SK_RSA k)
+  | DSA    -> let k = dsa_gen_key 1024 in (PK_DSA k, SK_DSA k)
+  | ECDSA  -> let k = ec_gen_key ({curve = ECC_P256; point_compression = false}) in (PK_ECDSA k, SK_ECDSA k)
+  | RSAPSS -> failwith "Signature.genrepr: RSA-PSS unsupported"
+
+val gen: a:alg -> All (skey a)
+                     (requires (fun h -> m_contains rkeys h))
+                     (ensures  (fun h0 (s:result (skey a)) h1 ->
+			       modifies_one keyRegion h0 h1
+                               /\ modifies_rref keyRegion !{as_ref (as_rref rkeys)} h0 h1
+                               /\ m_contains rkeys h1
+			       /\ (is_V s ==>
+				 witnessed (generated (|a, fst (V.v s) |))
+				 /\ m_fresh (PK.log (fst (V.v s))) h0 h1 )))
+
+let rec gen a =
+  let pkr,skr = genrepr a in // Could be inlined
+  let keys = m_read rkeys in
+  match find_key pkr keys with
+  | Some _ -> gen a // retry until distinct. SZ: why not just throw an exception?
+  | None ->
+     let p = alloc_pubkey (Signed Seq.createEmpty) pkr in
+     let k = (| a, p |) in
+     let keys' = add_key keys k in
+     m_write rkeys keys';
+     witness rkeys (generated (|a, p|));
+     p, skr
+
+
+(* ------------------------------------------------------------------------ *)
+val leak: #a:alg -> s:skey a -> ST (public_repr * secret_repr)
+  (requires (fun _ -> True))
+  (ensures  (fun h0 r h1 ->
+	      modifies_one keyRegion h0 h1
+	      /\ modifies_rref keyRegion !{as_ref (as_rref (PK.log (fst s)))} h0 h1
+	      /\ is_Corrupt (m_sel h1 (PK.log (fst s)))
+	      /\ fst r = PK.repr (fst s)))     
+let leak #a (PK log pkr, skr) =
+  m_write log Corrupt; 
+  pkr, skr
+
+
+(* ------------------------------------------------------------------------ *)
+val coerce: #a:alg -> pkr:public_repr{sigAlg_of_public_repr pkr = a.core} -> skr:secret_repr{sigAlg_of_secret_repr skr = a.core} -> ST (skey a)
+  (requires (fun _ -> True))
+  (ensures (fun h0 s h1 ->
+           is_Corrupt (m_sel h1 (PK.log (fst s)))
+           /\ PK.repr (fst s) = pkr
+	   /\ snd s = skr))
+let coerce #a pkr skr =
+  alloc_pubkey Corrupt pkr, skr
+
+
+(* ------------------------------------------------------------------------ *)
+val endorse: #a:alg -> pkr:public_repr{sigAlg_of_public_repr pkr = a.core} -> ST pkey
+  (requires (fun _ -> True))
+  (ensures  (fun h0 k h1 -> 
+	     pkey_repr k = pkr
+             /\ (forall k'. generated k' h1 /\ pkey_repr k' = pkr ==> k = k')))
+let endorse #a pkr =
+  let keys = m_read rkeys in
+  match find_key pkr keys with
+  | Some k -> k
+  | None   -> (| a, alloc_pubkey Corrupt pkr |)
+
+
+#reset-options 
+#set-options "--initial_fuel 2 --max_fuel 2 --detail_errors"
+
+val test: bytes -> bytes -> All unit
+      (requires (fun h -> m_contains rkeys h))
+      (ensures (fun h0 _ h1 -> modifies (Set.singleton keyRegion) h0 h1))
+let test t0 t1 =
+  let a = Use (fun t -> True)
+	      RSASIG
+              [Hash SHA256; Hash SHA384]
+              false
+              false in
+  let a' = Use (fun t -> t = t1)
+              RSASIG
+              [Hash SHA256]
+              false
+              false in
+  let s = gen a in
+  let s' = gen a' in
+  let sigv0 = sign (Hash SHA256) s t0 in
+  let sigv1 = sign (Hash SHA256) s t1 in
+  //let sigv2 = sign (Hash SHA256) s' t0 in // should fail, can only sign t1
+  ()
